\documentclass [12pt,fleqn] {article}
\usepackage{polski}
\usepackage[utf8]{inputenc}
\usepackage{amsmath}

\setlength{\mathindent}{0cm}

\title{\textbf{TESTY}}
\thispagestyle{empty}
\pagestyle{empty}
\begin{document}
%\maketitle
\section*{Test 1}
\[n=2; a=1; b=3 \]
\[x_0=1; x_1=2; x_2=3\]
\[l_0=\prod\limits_{k=0;k\neq0}^2\frac{x-x_k}{x_0-x_k}=\frac{x-x_1}{x_0-x_1}*\frac{x-x_2}{x_0-x_2}=\frac{x-2}{-1}*\frac{x-3}{-2}=\frac{1}{2}x^2-\frac{5}{2}x+3\]
\[l_0(x_0)=l_0(1)=1; l_0(x_1)=l_0(2)=0; l_0(x_2)=l_0(2)=0;\]
\[l_1=\prod\limits_{k=0;k\neq1}^2\frac{x-x_k}{x_1-x_k}=\frac{x-x_0}{x_1-x_0}*\frac{x-x_1}{x_0-x_2}=\frac{x-1}{1}*\frac{x-3}{-1}=-x^2+4x-3\]
\[l_1(x_0)=l_1(1)=0; l_1(x_1)=l_1(2)=1; l_1(x_2)=l_1(2)=0;\]
\[l_2=\prod\limits_{k=0;k\neq2}^2\frac{x-x_k}{x_2-x_k}=\frac{x-x_0}{x_2-x_0}*\frac{x-x_2}{x_0-x_1}=\frac{x-1}{2}*\frac{x-2}{1}=\frac{1}{2}x^2-\frac{3}{2}x+1\]
\[l_2(x_0)=l_2(1)=0; l_2(x_1)=l_2(2)=0; l_2(x_2)=l_2(2)=1;\]
\[1*\]
\[A_0=1; A_1=4; A_2=9\]
\[L(x)=\sum\limits_{i=0}^2A_i*l_i(x)=1(\frac{1}{2}x^2-\frac{5}{2}x+3)+4(x^2+4x-3)+9(\frac{1}{2}x^2-\frac{3}{2}x+1)=x^2\]
\[2*\]
\[A_0=2; A_1=1; A_2=3\]
\[L(x)=\sum\limits_{i=0}^2A_i*l_i(x)=2(\frac{1}{2}x^2-\frac{5}{2}x+3)+1(x^2+4x-3)+3(\frac{1}{2}x^2-\frac{3}{2}x+1)=\frac{3}{2}x^2-\frac{11}{2}x+6\]
\newpage
\section*{Test 2}
\[n=1; a=1; b=2\]
\[x_0=1; x_1=2\]
\[l_0=\prod\limits_{k=0;k\neq0}^1\frac{x-x_k}{x_0-x_k}=\frac{x-x_1}{x_0-x_1}=\frac{x-2}{-1}=-x+2\]
\[l_0(x_0)=l_0(1)=1; l_0(x_1)=l_0(2)=0\]
\[l_0=\prod\limits_{k=0;k\neq1}^1\frac{x-x_k}{x_1-x_k}=\frac{x-x_0}{x_1-x_0}=\frac{x-1}{1}=x-1\]
\[l_1(x_0)=l_1(1)=0; l_1(x_1)=l_1(2)=1\]
\[1*\]
\[A_0=f(x_0)=f(1)=1; A_1=f(x_1)=f(2)=2\]
\[L(x)=\sum\limits_{i=0}^1A_i*l_i(x)=1(-x+2)+2(x-1)=x\]
\[2*\]
\[A_0=f(x_0)=f(1)=0; A_1=f(x_1)=f(2)=0\]
\[L(x)=\sum\limits_{i=0}^1A_i*l_i(x)=0(-x+2)+0(x-1)=0\]
\[3*\]
\[A_0=f(x_0)=f(1)=3; A_1=f(x_1)=f(2)=1\]
\[L(x)=\sum\limits_{i=0}^1A_i*l_i(x)=3(-x+2)+1(x-1)=-2x+5\]
\newpage
\section*{Test 3}
\[n=3; a=0; b=6\]
\[x_0=0; x_1=2; x_2=4; x_3=6\]
\[l_0=\prod\limits_{k=0;k\neq0}^3\frac{x-x_k}{x_0-x_k}=\frac{x-x_1}{x_0-x_1}*\frac{x-x_2}{x_0-x_2}*\frac{x-x_3}{x_0-x_3}=\]\[=\frac{x-2}{-2}*\frac{x-4}{-4}*\frac{x-6}{-6}=-\frac{1}{48}x^3+\frac{1}{4}x^2-\frac{44}{48}x+1\]
\[l_1=\prod\limits_{k=0;k\neq1}^3\frac{x-x_k}{x_1-x_k}=\frac{x-x_0}{x_1-x_0}*\frac{x-x_2}{x_1-x_2}*\frac{x-x_3}{x_1-x_3}=\]\[=\frac{x-0}{2}*\frac{x-4}{-2}*\frac{x-6}{-4}=\frac{1}{16}x^3-\frac{5}{8}x^2+\frac{3}{2}x\]
\[l_2=\prod\limits_{k=0;k\neq2}^3\frac{x-x_k}{x_2-x_k}=\frac{x-x_0}{x_2-x_0}*\frac{x-x_1}{x_2-x_1}*\frac{x-x_3}{x_2-x_3}=\]\[=\frac{x-0}{4}*\frac{x-2}{2}*\frac{x-6}{-2}=-\frac{1}{16}x^3+\frac{1}{2}x^2+\frac{3}{4}x\]
\[l_3=\prod\limits_{k=0;k\neq3}^3\frac{x-x_k}{x_3-x_k}=\frac{x-x_0}{x_3-x_0}*\frac{x-x_1}{x_3-x_1}*\frac{x-x_2}{x_3-x_2}=\]\[=\frac{x-0}{6}*\frac{x-2}{4}*\frac{x-6}{2}=\frac{1}{48}x^3-\frac{1}{6}x^2+\frac{1}{4}x\]
\[1*\]
\[A_0=f(x_0)=f(0)=0; A_1=f(x_1)=f(2)=0;\] \[ A_2=f(x_2)=f(4)=0; A_3=f(x_3)=f(6)=0;\]
\[L(x)=\sum\limits_{i=0}^3A_i*l_i(x)=0\]
\end{document}